lib/Binary.v
@@ -1,6 +1,7 @@
 Require Import List.
 Require Import Arith.
 Require Import Nat.
+Require Import Ascii.
 
 Fixpoint take_rec (acc: list bool) c xs :=
   match c with
@@ -25,13 +26,48 @@ Definition add_zeroes bin len :=
   if ge_dec (length bin) len then
     bin
   else
-    add_zeroes_rec bin len.
+    add_zeroes_rec bin (len - (length bin)).
 
-(* Fixpoint nat_to_binary_rec n := *)
-(*   match n with *)
-(*     | O => nil *)
-(*     | _ => (modulo n 2 = 1) :: nat_to_binary_rec (div2 n) *)
-(*   end. *)
+Fixpoint nat_to_binary_rec fuel n :=
+  match fuel with
+    | 0 => nil
+    | S fuel =>
+  match n with
+    | O => nil
+    | _ => (eqb (modulo n 2) 1) :: nat_to_binary_rec fuel (div2 n)
+  end
+  end.
 
-(* Definition nat_to_binary n := *)
-(*   rev (nat_to_binary_rec n). *)
+Definition nat_to_binary n :=
+  rev (nat_to_binary_rec n n).
+
+Fixpoint binary_to_nat_rec bin :=
+  match bin with
+    | nil => 0
+    | hd::bin =>
+      (match hd with
+         | true => 1
+         | false => 0
+       end) + 2 * (binary_to_nat_rec bin)
+  end.
+
+Definition binary_to_nat bin :=
+  binary_to_nat_rec (List.rev bin).
+
+Definition int_to_binary i :=
+  add_zeroes (nat_to_binary i) 31.
+
+Definition binary_to_int bin :=
+  match take 31 bin with
+    | Some (bin, rest) => Some (binary_to_nat bin, rest)
+    | None => None
+  end.
+
+Definition ascii_to_binary a :=
+  add_zeroes (nat_to_binary (nat_of_ascii a)) 8.
+
+Definition binary_to_ascii bin :=
+  match take 8 bin with
+    | Some (bin, rest) => Some (ascii_of_nat (binary_to_nat bin), rest)
+    | None => None
+  end.
